---
title: Formalisation of the Symmetry Book
---

```agda
{-# OPTIONS --without-K --exact-split --safe #-}

module foundations.04-inductive-types where

open import foundations.03-natural-numbers public
```

## The unit type

```agda
data unit : UU lzero where
  star : unit

ind-unit : {l : Level} {P : unit â†’ UU l} â†’ P star â†’ ((x : unit) â†’ P x)
ind-unit p star = p

terminal-map : {l : Level} {A : UU l} â†’ A â†’ unit
terminal-map a = star

raise-unit : (l : Level) â†’ UU l
raise-unit l = raise l unit

raise-star : {l : Level} â†’ raise l unit
raise-star = map-raise star
```

## The empty type

```agda
data empty : UU lzero where

ğŸ˜ = empty

ind-empty : {l : Level} {P : empty â†’ UU l} â†’ ((x : empty) â†’ P x)
ind-empty ()

ex-falso : {l : Level} {A : UU l} â†’ empty â†’ A
ex-falso = ind-empty

raise-empty : (l : Level) â†’ UU l
raise-empty l = raise l empty

Â¬ : {l : Level} â†’ UU l â†’ UU l
Â¬ A = A â†’ empty

is-empty : {l : Level} â†’ UU l â†’ UU l
is-empty = Â¬

is-nonempty : {l : Level} â†’ UU l â†’ UU l
is-nonempty A = Â¬ (is-empty A)

functor-neg : {l1 l2 : Level} {P : UU l1} {Q : UU l2} â†’
  (P â†’ Q) â†’ (Â¬ Q â†’ Â¬ P)
functor-neg f nq p = nq (f p)
```

## The booleans

```agda
data bool : UU lzero where
  true false : bool

{-# BUILTIN BOOL bool #-}
{-# BUILTIN TRUE  true  #-}
{-# BUILTIN FALSE false #-}
```

### The boolean operators

```agda
neg-bool : bool â†’ bool
neg-bool true = false
neg-bool false = true

conjunction-bool : bool â†’ (bool â†’ bool)
conjunction-bool true true = true
conjunction-bool true false = false
conjunction-bool false true = false
conjunction-bool false false = false

disjunction-bool : bool â†’ (bool â†’ bool)
disjunction-bool true true = true
disjunction-bool true false = true
disjunction-bool false true = true
disjunction-bool false false = false
```

## Coproducts

```agda
data coprod {l1 l2 : Level} (A : UU l1) (B : UU l2) : UU (l1 âŠ” l2)  where
  inl : A â†’ coprod A B
  inr : B â†’ coprod A B

ind-coprod :
  {l1 l2 l3 : Level} {A : UU l1} {B : UU l2} (C : coprod A B â†’ UU l3) â†’
  ((x : A) â†’ C (inl x)) â†’ ((y : B) â†’ C (inr y)) â†’
  (t : coprod A B) â†’ C t
ind-coprod C f g (inl x) = f x
ind-coprod C f g (inr x) = g x

map-coprod :
  {l1 l2 l1' l2' : Level} {A : UU l1} {B : UU l2} {A' : UU l1'} {B' : UU l2'} â†’
  (A â†’ A') â†’ (B â†’ B') â†’ coprod A B â†’ coprod A' B'
map-coprod f g (inl x) = inl (f x)
map-coprod f g (inr y) = inr (g y)

map-right-unit-law-coprod-is-empty :
  {l1 l2 : Level} (A : UU l1) (B : UU l2) â†’ is-empty B â†’ coprod A B â†’ A
map-right-unit-law-coprod-is-empty A B nb (inl a) = a
map-right-unit-law-coprod-is-empty A B nb (inr b) = ex-falso (nb b)

map-left-unit-law-coprod-is-empty :
  {l1 l2 : Level} (A : UU l1) (B : UU l2) â†’ is-empty A â†’ coprod A B â†’ B
map-left-unit-law-coprod-is-empty A B na (inl a) = ex-falso (na a)
map-left-unit-law-coprod-is-empty A B na (inr b) = b
```

## Dependent pair types

```agda
record Î£ {l1 l2} (A : UU l1) (B : A â†’ UU l2) : UU (l1 âŠ” l2) where
  constructor pair
  field
    pr1 : A
    pr2 : B pr1

open Î£ public

{-# BUILTIN SIGMA Î£ #-}

ind-Î£ :
  {l1 l2 l3 : Level} {A : UU l1} {B : A â†’ UU l2} {C : Î£ A B â†’ UU l3} â†’
  ((x : A) (y : B x) â†’ C (pair x y)) â†’ ((t : Î£ A B) â†’ C t)
ind-Î£ f (pair x y) = f x y

ev-pair :
  {l1 l2 l3 : Level} {A : UU l1} {B : A â†’ UU l2} {C : Î£ A B â†’ UU l3} â†’
  ((t : Î£ A B) â†’ C t) â†’ (x : A) (y : B x) â†’ C (pair x y)
ev-pair f x y = f (pair x y)
```

## Cartesian products

```agda
prod : {l1 l2 : Level} (A : UU l1) (B : UU l2) â†’ UU (l1 âŠ” l2)
prod A B = Î£ A (Î» a â†’ B)

pair' :
  {l1 l2 : Level} {A : UU l1} {B : UU l2} â†’ A â†’ B â†’ prod A B
pair' = pair

_Ã—_ :  {l1 l2 : Level} (A : UU l1) (B : UU l2) â†’ UU (l1 âŠ” l2)
A Ã— B = prod A B

map-prod :
  {l1 l2 l3 l4 : Level} {A : UU l1} {B : UU l2} {C : UU l3} {D : UU l4}
  (f : A â†’ C) (g : B â†’ D) â†’ (A Ã— B) â†’ (C Ã— D)
pr1 (map-prod f g (pair a b)) = f a
pr2 (map-prod f g (pair a b)) = g b
```

## The type of integers

```agda
â„¤ : UU lzero
â„¤ = coprod â„• (coprod unit â„•)
```

- Inclusion of the negative integers

```agda
in-neg : â„• â†’ â„¤
in-neg n = inl n
```

- Negative one

```agda
neg-one-â„¤ : â„¤
neg-one-â„¤ = in-neg zero-â„•
```

- Zero

```agda
zero-â„¤ : â„¤
zero-â„¤ = inr (inl star)
```

- One

```agda
one-â„¤ : â„¤
one-â„¤ = inr (inr zero-â„•)
```

- Inclusion of the positive integers

```agda
in-pos : â„• â†’ â„¤
in-pos n = inr (inr n)
```

- Inclusion of the natural numbers

```agda
int-â„• : â„• â†’ â„¤
int-â„• zero-â„• = zero-â„¤
int-â„• (succ-â„• n) = in-pos n
```

- Induction principle on the type of integers

```agda
ind-â„¤ :
  {l : Level} (P : â„¤ â†’ UU l) â†’
  P neg-one-â„¤ â†’ ((n : â„•) â†’ P (inl n) â†’ P (inl (succ-â„• n))) â†’
  P zero-â„¤ â†’
  P one-â„¤ â†’ ((n : â„•) â†’ P (inr (inr (n))) â†’ P (inr (inr (succ-â„• n)))) â†’
  (k : â„¤) â†’ P k
ind-â„¤ P p-1 p-S p0 p1 pS (inl zero-â„•) = p-1
ind-â„¤ P p-1 p-S p0 p1 pS (inl (succ-â„• x)) =
  p-S x (ind-â„¤ P p-1 p-S p0 p1 pS (inl x))
ind-â„¤ P p-1 p-S p0 p1 pS (inr (inl star)) = p0
ind-â„¤ P p-1 p-S p0 p1 pS (inr (inr zero-â„•)) = p1
ind-â„¤ P p-1 p-S p0 p1 pS (inr (inr (succ-â„• x))) =
  pS x (ind-â„¤ P p-1 p-S p0 p1 pS (inr (inr (x))))
```

- The successor and predecessor functions on â„¤

```agda
succ-â„¤ : â„¤ â†’ â„¤
succ-â„¤ (inl zero-â„•) = zero-â„¤
succ-â„¤ (inl (succ-â„• x)) = inl x
succ-â„¤ (inr (inl star)) = one-â„¤
succ-â„¤ (inr (inr x)) = inr (inr (succ-â„• x))

pred-â„¤ : â„¤ â†’ â„¤
pred-â„¤ (inl x) = inl (succ-â„• x)
pred-â„¤ (inr (inl star)) = inl zero-â„•
pred-â„¤ (inr (inr zero-â„•)) = inr (inl star)
pred-â„¤ (inr (inr (succ-â„• x))) = inr (inr x)
```

### Arithmetic operations on the integers

- Addition on â„¤

```agda
add-â„¤ : â„¤ â†’ â„¤ â†’ â„¤
add-â„¤ (inl zero-â„•) l = pred-â„¤ l
add-â„¤ (inl (succ-â„• x)) l = pred-â„¤ (add-â„¤ (inl x) l)
add-â„¤ (inr (inl star)) l = l
add-â„¤ (inr (inr zero-â„•)) l = succ-â„¤ l
add-â„¤ (inr (inr (succ-â„• x))) l = succ-â„¤ (add-â„¤ (inr (inr x)) l)

add-â„¤' : â„¤ â†’ â„¤ â†’ â„¤
add-â„¤' x y = add-â„¤ y x
```

- The negative of an integer

```agda
neg-â„¤ : â„¤ â†’ â„¤
neg-â„¤ (inl x) = inr (inr x)
neg-â„¤ (inr (inl star)) = inr (inl star)
neg-â„¤ (inr (inr x)) = inl x
```

- Multiplication of integers

We give two definitions of multiplication on â„¤

```agda
mul-â„¤ : â„¤ â†’ â„¤ â†’ â„¤
mul-â„¤ (inl zero-â„•) l = neg-â„¤ l
mul-â„¤ (inl (succ-â„• x)) l = add-â„¤ (neg-â„¤ l) (mul-â„¤ (inl x) l)
mul-â„¤ (inr (inl star)) l = zero-â„¤
mul-â„¤ (inr (inr zero-â„•)) l = l
mul-â„¤ (inr (inr (succ-â„• x))) l = add-â„¤ l (mul-â„¤ (inr (inr x)) l)

mul-â„¤' : â„¤ â†’ â„¤ â†’ â„¤
mul-â„¤' x y = mul-â„¤ y x

explicit-mul-â„¤ : â„¤ â†’ â„¤ â†’ â„¤
explicit-mul-â„¤ (inl x) (inl y) = int-â„• (mul-â„• (succ-â„• x) (succ-â„• y))
explicit-mul-â„¤ (inl x) (inr (inl star)) = zero-â„¤
explicit-mul-â„¤ (inl x) (inr (inr y)) =
  neg-â„¤ (int-â„• (mul-â„• (succ-â„• x) (succ-â„• y)))
explicit-mul-â„¤ (inr (inl star)) (inl y) = zero-â„¤
explicit-mul-â„¤ (inr (inr x)) (inl y) =
  neg-â„¤ (int-â„• (mul-â„• (succ-â„• x) (succ-â„• y)))
explicit-mul-â„¤ (inr (inl star)) (inr (inl star)) = zero-â„¤
explicit-mul-â„¤ (inr (inl star)) (inr (inr y)) = zero-â„¤
explicit-mul-â„¤ (inr (inr x)) (inr (inl star)) = zero-â„¤
explicit-mul-â„¤ (inr (inr x)) (inr (inr y)) = int-â„• (mul-â„• (succ-â„• x) (succ-â„• y))

explicit-mul-â„¤' : â„¤ â†’ â„¤ â†’ â„¤
explicit-mul-â„¤' x y = explicit-mul-â„¤ y x
```

##  Logical equivalence

```agda
_â†”_ : {l1 l2 : Level} â†’ UU l1 â†’ UU l2 â†’ UU (l1 âŠ” l2)
A â†” B = (A â†’ B) Ã— (B â†’ A)

_âˆ˜iff_ :
  {l1 l2 l3 : Level} {A : UU l1} {B : UU l2} {C : UU l3} â†’
  (B â†” C) â†’ (A â†” B) â†’ (A â†” C)
pr1 (pair g1 g2 âˆ˜iff pair f1 f2) = g1 âˆ˜ f1
pr2 (pair g1 g2 âˆ˜iff pair f1 f2) = f2 âˆ˜ g2
```

## Double negation

```agda
Â¬Â¬ : {l : Level} â†’ UU l â†’ UU l
Â¬Â¬ P = Â¬ (Â¬ P)

Â¬Â¬Â¬ : {l : Level} â†’ UU l â†’ UU l
Â¬Â¬Â¬ P = Â¬ (Â¬ (Â¬ P))

intro-dn : {l : Level} {P : UU l} â†’ P â†’ Â¬Â¬ P
intro-dn p f = f p

functor-dn : {l1 l2 : Level} {P : UU l1} {Q : UU l2} â†’
  (P â†’ Q) â†’ (Â¬Â¬ P â†’ Â¬Â¬ Q)
functor-dn f = functor-neg (functor-neg f)

```

```agda
no-fixed-points-neg :
  {l : Level} (A : UU l) â†’ Â¬ ((A â†’ Â¬ A) Ã— (Â¬ A â†’ A))
no-fixed-points-neg A (pair f g) =
  ( Î» (h : Â¬ A) â†’ h (g h)) (Î» (a : A) â†’ f a a)
```

In this exercise we were asked to show that $A + Â¬A$ implies $Â¬Â¬A â†’ A$.
We get double negation elimination for the types that are  decidable.

```agda
dn-elim-is-decidable :
  {l : Level} (P : UU l) â†’ coprod P (Â¬ P) â†’ (Â¬Â¬ P â†’ P)
dn-elim-is-decidable P (inl x) p = x
dn-elim-is-decidable P (inr x) p = ex-falso (p x)

dn-is-decidable : {l : Level} {P : UU l} â†’ Â¬Â¬ (coprod P (Â¬ P))
dn-is-decidable {P = P} f =
  functor-neg (inr {A = P} {B = Â¬ P}) f
    ( functor-neg (inl {A = P} {B = Â¬ P}) f)

dn-dn-elim : {l : Level} {P : UU l} â†’ Â¬Â¬ (Â¬Â¬ P â†’ P)
dn-dn-elim {P = P} f =
  ( Î» (np : Â¬ P) â†’ f (Î» (nnp : Â¬Â¬ P) â†’ ex-falso (nnp np)))
    ( Î» (p : P) â†’ f (Î» (nnp : Â¬Â¬ P) â†’ p))
```

## Double negations of classical laws

```agda
Peirces-law :
  {l1 l2 : Level} {P : UU l1} {Q : UU l2} â†’
  Â¬Â¬ (((P â†’ Q) â†’ P) â†’ P)
Peirces-law {P = P} {Q} f =
  ( Î» (np : Â¬ P) â†’ f (Î» h â†’ h (Î» p â†’ ex-falso (np p))))
  ( Î» (p : P) â†’ f (Î» h â†’ p))

dn-linearity-implication :
  {l1 l2 : Level} {P : UU l1} {Q : UU l2} â†’
  Â¬Â¬ (coprod (P â†’ Q) (Q â†’ P))
dn-linearity-implication {P = P} {Q = Q} f =
  ( Î» (np : Â¬ P) â†’
    functor-neg (inl {A = P â†’ Q} {B = Q â†’ P}) f (Î» p â†’ ex-falso (np p)))
    ( Î» (p : P) â†’
      functor-neg (inr {A = P â†’ Q} {B = Q â†’ P}) f (Î» q â†’ p))
```

## Cases of double negation elimination

```agda
dn-elim-neg : {l : Level} (P : UU l) â†’ Â¬Â¬Â¬ P â†’ Â¬ P
dn-elim-neg P f p = f (Î» g â†’ g p)

dn-extend :
  {l1 l2 : Level} {P : UU l1} {Q : UU l2} â†’
  (P â†’ Â¬Â¬ Q) â†’ (Â¬Â¬ P â†’ Â¬Â¬ Q)
dn-extend {P = P} {Q = Q} f = dn-elim-neg (Â¬ Q) âˆ˜ (functor-dn f)

dn-elim-exp :
  {l1 l2 : Level} {P : UU l1} {Q : UU l2} â†’
  Â¬Â¬ (P â†’ Â¬Â¬ Q) â†’ (P â†’ Â¬Â¬ Q)
dn-elim-exp {P = P} {Q = Q} f p =
  dn-elim-neg (Â¬ Q) (functor-dn (Î» (g : P â†’ Â¬Â¬ Q) â†’ g p) f)

dn-elim-prod :
  {l1 l2 : Level} {P : UU l1} {Q : UU l2} â†’
  Â¬Â¬ ((Â¬Â¬ P) Ã— (Â¬Â¬ Q)) â†’ (Â¬Â¬ P) Ã— (Â¬Â¬ Q)
pr1 (dn-elim-prod {P = P} {Q = Q} f) = dn-elim-neg (Â¬ P) (functor-dn pr1 f)
pr2 (dn-elim-prod {P = P} {Q = Q} f) = dn-elim-neg (Â¬ Q) (functor-dn pr2 f)
```

## Lists

```agda
data list {l : Level} (A : UU l) : UU l where
  nil : list A
  cons : A â†’ list A â†’ list A

in-list : {l : Level} {A : UU l} â†’ A â†’ list A
in-list a = cons a nil
```

## Operations on lists

```agda
fold-list :
  {l1 l2 : Level} {A : UU l1} {B : UU l2} (b : B) (Î¼ : A â†’ (B â†’ B)) â†’
  list A â†’ B
fold-list b Î¼ nil = b
fold-list b Î¼ (cons a l) = Î¼ a (fold-list b Î¼ l)

length-list : {l : Level} {A : UU l} â†’ list A â†’ â„•
length-list = fold-list zero-â„• (Î» a â†’ succ-â„•)

sum-list-â„• : list â„• â†’ â„•
sum-list-â„• = fold-list zero-â„• add-â„•

product-list-â„• : list â„• â†’ â„•
product-list-â„• = fold-list one-â„• mul-â„•

concat-list : {l : Level} {A : UU l} â†’ list A â†’ (list A â†’ list A)
concat-list {l} {A} = fold-list id (Î» a f â†’ (cons a) âˆ˜ f)

flatten-list : {l : Level} {A : UU l} â†’ list (list A) â†’ list A
flatten-list = fold-list nil concat-list

reverse-list : {l : Level} {A : UU l} â†’ list A â†’ list A
reverse-list nil = nil
reverse-list (cons a l) = concat-list (reverse-list l) (in-list a)
```
