---
title: Formalisation of the Symmetry Book
---

```agda
{-# OPTIONS --without-K --exact-split --safe #-}

module foundations.06-universes where

import foundations.05-identity-types
open foundations.05-identity-types public

--------------------------------------------------------------------------------

-- Section 6.3 Observational equality on the natural numbers

-- Definition 6.3.1

Eq-ℕ : ℕ → ℕ → UU lzero
Eq-ℕ zero-ℕ zero-ℕ = unit
Eq-ℕ zero-ℕ (succ-ℕ n) = empty
Eq-ℕ (succ-ℕ m) zero-ℕ = empty
Eq-ℕ (succ-ℕ m) (succ-ℕ n) = Eq-ℕ m n

Eq-ℤ : ℤ → ℤ → UU lzero
Eq-ℤ (inl x) (inl y) = Eq-ℕ x y
Eq-ℤ (inl x) (inr y) = empty
Eq-ℤ (inr x) (inl y) = empty
Eq-ℤ (inr (inl x)) (inr (inl y)) = unit
Eq-ℤ (inr (inl x)) (inr (inr y)) = empty
Eq-ℤ (inr (inr x)) (inr (inl y)) = empty
Eq-ℤ (inr (inr x)) (inr (inr y)) = Eq-ℕ x y

-- Lemma 6.3.2

refl-Eq-ℕ : (n : ℕ) → Eq-ℕ n n
refl-Eq-ℕ zero-ℕ = star
refl-Eq-ℕ (succ-ℕ n) = refl-Eq-ℕ n

refl-Eq-ℤ : (x : ℤ) → Eq-ℤ x x
refl-Eq-ℤ (inl x) = refl-Eq-ℕ x
refl-Eq-ℤ (inr (inl x)) = star
refl-Eq-ℤ (inr (inr x)) = refl-Eq-ℕ x

-- Proposition 6.3.3

Eq-eq-ℕ : {x y : ℕ} → Id x y → Eq-ℕ x y
Eq-eq-ℕ {x} {.x} refl = refl-Eq-ℕ x

eq-Eq-ℕ : (x y : ℕ) → Eq-ℕ x y → Id x y
eq-Eq-ℕ zero-ℕ zero-ℕ e = refl
eq-Eq-ℕ (succ-ℕ x) (succ-ℕ y) e = ap succ-ℕ (eq-Eq-ℕ x y e)

Eq-eq-ℤ : {x y : ℤ} → Id x y → Eq-ℤ x y
Eq-eq-ℤ {x} {.x} refl = refl-Eq-ℤ x

eq-Eq-ℤ : (x y : ℤ) → Eq-ℤ x y → Id x y
eq-Eq-ℤ (inl x) (inl y) e = ap inl (eq-Eq-ℕ x y e)
eq-Eq-ℤ (inr (inl star)) (inr (inl star)) e = refl
eq-Eq-ℤ (inr (inr x)) (inr (inr y)) e = ap (inr ∘ inr) (eq-Eq-ℕ x y e)

--------------------------------------------------------------------------------

-- Section 6.4 Peano's seventh and eighth axioms

-- Theorem 6.4.1

is-injective : {l1 l2 : Level} {A : UU l1} {B : UU l2} → (A → B) → UU (l1 ⊔ l2)
is-injective {l1} {l2} {A} {B} f = ({x y : A} → Id (f x) (f y) → Id x y)

is-not-injective :
  {l1 l2 : Level} {A : UU l1} {B : UU l2} (f : A → B) → UU (l1 ⊔ l2)
is-not-injective f = ¬ (is-injective f)

is-injective-id : {l1 : Level} {A : UU l1} → is-injective (id {A = A})
is-injective-id p = p

module _
  {l1 l2 l3 : Level} {A : UU l1} {B : UU l2} {C : UU l3}
  where
  
  is-injective-is-injective-comp :
    (f : A → C) (g : B → C) (h : A → B) (H : (a : A) → Id (f a) (g (h a))) →
    is-injective f → is-injective h
  is-injective-is-injective-comp f g h H is-inj-f {x} {x'} p =
    is-inj-f {x} {x'} ((H x) ∙ ((ap g p) ∙ (inv (H x'))))

  is-injective-comp :
    (f : A → C) (g : B → C) (h : A → B) (H : (a : A) → Id (f a) (g (h a))) →
    is-injective h → is-injective g → is-injective f
  is-injective-comp f g h H is-inj-h is-inj-g {x} {x'} p =
    is-inj-h (is-inj-g ((inv (H x)) ∙ (p ∙ (H x'))))

  is-injective-comp' :
    {g : B → C} {h : A → B} →
    is-injective h → is-injective g → is-injective (g ∘ h)
  is-injective-comp' {g} {h} H G =
    is-injective-comp (g ∘ h) g h (λ x → refl) H G

is-injective-succ-ℕ : is-injective succ-ℕ
is-injective-succ-ℕ {x} {y} e = eq-Eq-ℕ x y (Eq-eq-ℕ e)

is-injective-succ-ℤ : is-injective succ-ℤ
is-injective-succ-ℤ {x} {y} p =
  inv (isretr-pred-ℤ x) ∙ (ap pred-ℤ p ∙ isretr-pred-ℤ y)

Peano-7 :
  (x y : ℕ) → (Id x y) ↔ (Id (succ-ℕ x) (succ-ℕ y))
pr1 (Peano-7 x y) = ap succ-ℕ
pr2 (Peano-7 x y) = is-injective-succ-ℕ

-- Theorem 6.4.2

is-zero-ℕ : ℕ → UU lzero
is-zero-ℕ n = Id n zero-ℕ

is-zero-ℕ' : ℕ → UU lzero
is-zero-ℕ' n = Id zero-ℕ n

is-successor-ℕ : ℕ → UU lzero
is-successor-ℕ n = Σ ℕ (λ y → Id n (succ-ℕ y))

is-nonzero-ℕ : ℕ → UU lzero
is-nonzero-ℕ n = ¬ (is-zero-ℕ n)

is-one-ℕ : ℕ → UU lzero
is-one-ℕ n = Id n one-ℕ

is-one-ℕ' : ℕ → UU lzero
is-one-ℕ' n = Id one-ℕ n

is-not-one-ℕ : ℕ → UU lzero
is-not-one-ℕ n = ¬ (is-one-ℕ n)

is-not-one-ℕ' : ℕ → UU lzero
is-not-one-ℕ' n = ¬ (is-one-ℕ' n)

Peano-8 : (x : ℕ) → is-nonzero-ℕ (succ-ℕ x)
Peano-8 x = Eq-eq-ℕ

is-nonzero-succ-ℕ : (x : ℕ) → is-nonzero-ℕ (succ-ℕ x)
is-nonzero-succ-ℕ = Peano-8

is-nonzero-is-successor-ℕ : {x : ℕ} → is-successor-ℕ x → is-nonzero-ℕ x
is-nonzero-is-successor-ℕ {.succ-ℕ x} (pair x refl) = Peano-8 x

is-successor-is-nonzero-ℕ : {x : ℕ} → is-nonzero-ℕ x → is-successor-ℕ x
is-successor-is-nonzero-ℕ {zero-ℕ} H = ex-falso (H refl)
pr1 (is-successor-is-nonzero-ℕ {succ-ℕ x} H) = x
pr2 (is-successor-is-nonzero-ℕ {succ-ℕ x} H) = refl

is-nonzero-one-ℕ : is-nonzero-ℕ one-ℕ
is-nonzero-one-ℕ = Peano-8 zero-ℕ

is-not-one-zero-ℕ : is-not-one-ℕ zero-ℕ
is-not-one-zero-ℕ = is-nonzero-one-ℕ ∘ inv

is-not-one-two-ℕ : is-not-one-ℕ two-ℕ
is-not-one-two-ℕ = Eq-eq-ℕ

has-no-fixed-points-succ-ℕ : (x : ℕ) → ¬ (Id (succ-ℕ x) x)
has-no-fixed-points-succ-ℕ zero-ℕ = is-nonzero-succ-ℕ zero-ℕ
has-no-fixed-points-succ-ℕ (succ-ℕ x) p =
  has-no-fixed-points-succ-ℕ x (is-injective-succ-ℕ p)

--------------------------------------------------------------------------------

-- Exercises

-- Exercise 6.1

-- Exercise 6.1 (a)

is-injective-add-ℕ' : (k : ℕ) → is-injective (add-ℕ' k)
is-injective-add-ℕ' zero-ℕ = id
is-injective-add-ℕ' (succ-ℕ k) p = is-injective-add-ℕ' k (is-injective-succ-ℕ p)

is-injective-add-ℤ' : (x : ℤ) → is-injective (add-ℤ' x)
is-injective-add-ℤ' x {y} {z} p =
  ( inv (isretr-add-neg-ℤ' x y)) ∙
  ( ( ap (add-ℤ' (neg-ℤ x)) p) ∙
    ( isretr-add-neg-ℤ' x z))

is-injective-add-ℕ : (k : ℕ) → is-injective (add-ℕ k)
is-injective-add-ℕ k {x} {y} p =
  is-injective-add-ℕ' k (commutative-add-ℕ x k ∙ (p ∙ commutative-add-ℕ k y))

is-injective-add-ℤ : (x : ℤ) → is-injective (add-ℤ x)
is-injective-add-ℤ x {y} {z} p =
  ( inv (isretr-add-neg-ℤ x y)) ∙
  ( ( ap (add-ℤ (neg-ℤ x)) p) ∙
    ( isretr-add-neg-ℤ x z))

is-injective-mul-succ-ℕ' :
  (k : ℕ) → is-injective (mul-ℕ' (succ-ℕ k))
is-injective-mul-succ-ℕ' k {zero-ℕ} {zero-ℕ} p = refl
is-injective-mul-succ-ℕ' k {succ-ℕ m} {succ-ℕ n} p =
  ap succ-ℕ
    ( is-injective-mul-succ-ℕ' k {m} {n}
      ( is-injective-add-ℕ'
        ( succ-ℕ k)
        ( ( inv (left-successor-law-mul-ℕ m (succ-ℕ k))) ∙
          ( ( p) ∙
            ( left-successor-law-mul-ℕ n (succ-ℕ k))))))

is-injective-mul-ℕ' :
  (k : ℕ) → is-nonzero-ℕ k → is-injective (mul-ℕ' k)
is-injective-mul-ℕ' k H p with
  is-successor-is-nonzero-ℕ H
... | pair l refl = is-injective-mul-succ-ℕ' l p

is-injective-mul-succ-ℕ :
  (k : ℕ) → is-injective (mul-ℕ (succ-ℕ k))
is-injective-mul-succ-ℕ k {m} {n} p =
  is-injective-mul-succ-ℕ' k
    ( ( commutative-mul-ℕ m (succ-ℕ k)) ∙
      ( p ∙ commutative-mul-ℕ (succ-ℕ k) n))

is-injective-mul-ℕ :
  (k : ℕ) → is-nonzero-ℕ k → is-injective (mul-ℕ k)
is-injective-mul-ℕ k H p with
  is-successor-is-nonzero-ℕ H
... | pair l refl = is-injective-mul-succ-ℕ l p

is-nonzero-mul-ℕ :
  (x y : ℕ) → is-nonzero-ℕ x → is-nonzero-ℕ y → is-nonzero-ℕ (mul-ℕ x y)
is-nonzero-mul-ℕ x y H K p =
  K (is-injective-mul-ℕ x H (p ∙ (inv (right-zero-law-mul-ℕ x))))

-- We conclude that y = 1 if (x+1)y = x+1

is-one-is-right-unit-mul-ℕ :
  (x y : ℕ) → Id (mul-ℕ (succ-ℕ x) y) (succ-ℕ x) → is-one-ℕ y
is-one-is-right-unit-mul-ℕ x y p =
  is-injective-mul-succ-ℕ x (p ∙ inv (right-unit-law-mul-ℕ (succ-ℕ x)))

is-one-is-left-unit-mul-ℕ :
  (x y : ℕ) → Id (mul-ℕ x (succ-ℕ y)) (succ-ℕ y) → is-one-ℕ x
is-one-is-left-unit-mul-ℕ x y p =
  is-injective-mul-succ-ℕ' y (p ∙ inv (left-unit-law-mul-ℕ (succ-ℕ y)))

-- Exercise 6.1 (b)

is-zero-right-is-zero-add-ℕ :
  (x y : ℕ) → is-zero-ℕ (add-ℕ x y) → is-zero-ℕ y
is-zero-right-is-zero-add-ℕ x zero-ℕ p = refl
is-zero-right-is-zero-add-ℕ x (succ-ℕ y) p = ex-falso (Peano-8 (add-ℕ x y) p)

is-zero-left-is-zero-add-ℕ :
  (x y : ℕ) → is-zero-ℕ (add-ℕ x y) → is-zero-ℕ x
is-zero-left-is-zero-add-ℕ x y p =
  is-zero-right-is-zero-add-ℕ y x ((commutative-add-ℕ y x) ∙ p)

is-zero-summand-is-zero-sum-ℕ :
  (x y : ℕ) → is-zero-ℕ (add-ℕ x y) → (is-zero-ℕ x) × (is-zero-ℕ y)
is-zero-summand-is-zero-sum-ℕ x y p =
  pair (is-zero-left-is-zero-add-ℕ x y p) (is-zero-right-is-zero-add-ℕ x y p)

is-zero-sum-is-zero-summand-ℕ :
  (x y : ℕ) → (is-zero-ℕ x) × (is-zero-ℕ y) → is-zero-ℕ (add-ℕ x y)
is-zero-sum-is-zero-summand-ℕ .zero-ℕ .zero-ℕ (pair refl refl) = refl

is-one-right-is-one-mul-ℕ :
  (x y : ℕ) → is-one-ℕ (mul-ℕ x y) → is-one-ℕ y
is-one-right-is-one-mul-ℕ zero-ℕ zero-ℕ p = p
is-one-right-is-one-mul-ℕ zero-ℕ (succ-ℕ y) p =
  ex-falso (Peano-8 zero-ℕ (inv p))
is-one-right-is-one-mul-ℕ (succ-ℕ x) zero-ℕ p =
  is-one-right-is-one-mul-ℕ x zero-ℕ p
is-one-right-is-one-mul-ℕ (succ-ℕ x) (succ-ℕ y) p =
  ap ( succ-ℕ)
     ( is-zero-right-is-zero-add-ℕ (mul-ℕ x (succ-ℕ y)) y
       ( is-injective-succ-ℕ p))

is-one-left-is-one-mul-ℕ :
  (x y : ℕ) → is-one-ℕ (mul-ℕ x y) → is-one-ℕ x
is-one-left-is-one-mul-ℕ x y p =
  is-one-right-is-one-mul-ℕ y x (commutative-mul-ℕ y x ∙ p)

-- Exercise 6.1 (c)

neq-add-ℕ :
  (m n : ℕ) → ¬ (Id m (add-ℕ m (succ-ℕ n)))
neq-add-ℕ (succ-ℕ m) n p =
  neq-add-ℕ m n
    ( ( is-injective-succ-ℕ p) ∙
      ( left-successor-law-add-ℕ m n))

neq-mul-ℕ :
  (m n : ℕ) → ¬ (Id (succ-ℕ m) (mul-ℕ (succ-ℕ m) (succ-ℕ (succ-ℕ n))))
neq-mul-ℕ m n p =
  neq-add-ℕ
    ( succ-ℕ m)
    ( add-ℕ (mul-ℕ m (succ-ℕ n)) n)
    ( ( p) ∙
      ( ( right-successor-law-mul-ℕ (succ-ℕ m) (succ-ℕ n)) ∙
        ( ap (add-ℕ (succ-ℕ m)) (left-successor-law-mul-ℕ m (succ-ℕ n)))))

-- Exercise 6.2

-- Exercise 6.2 (a)

Eq-bool : bool → bool → UU lzero
Eq-bool true true = unit
Eq-bool true false = empty
Eq-bool false true = empty
Eq-bool false false = unit

-- Exercise 6.2 (b)

refl-Eq-bool : (x : bool) → Eq-bool x x
refl-Eq-bool true = star
refl-Eq-bool false = star

Eq-eq-bool :
  {x y : bool} → Id x y → Eq-bool x y
Eq-eq-bool {x = x} refl = refl-Eq-bool x

eq-Eq-bool :
  {x y : bool} → Eq-bool x y → Id x y
eq-Eq-bool {true} {true} star = refl
eq-Eq-bool {false} {false} star = refl

-- Exercise 6.2 (c)

neq-neg-bool : (b : bool) → ¬ (Id b (neg-bool b))
neq-neg-bool true = Eq-eq-bool
neq-neg-bool false = Eq-eq-bool

neq-false-true-bool :
  ¬ (Id false true)
neq-false-true-bool = Eq-eq-bool

-- Exercise 6.3

leq-ℕ : ℕ → ℕ → UU lzero
leq-ℕ zero-ℕ m = unit
leq-ℕ (succ-ℕ n) zero-ℕ = empty
leq-ℕ (succ-ℕ n) (succ-ℕ m) = leq-ℕ n m

_≤-ℕ_ = leq-ℕ

data leq-ℕ' : ℕ → ℕ → UU lzero where
  refl-leq-ℕ' : (n : ℕ) → leq-ℕ' n n
  propagate-leq-ℕ' : {x y z : ℕ} → Id (succ-ℕ y) z → (leq-ℕ' x y) → (leq-ℕ' x z) 

-- Some trivialities that will be useful later

leq-zero-ℕ :
  (n : ℕ) → zero-ℕ ≤-ℕ n
leq-zero-ℕ n = star

is-zero-leq-zero-ℕ :
  (x : ℕ) → x ≤-ℕ zero-ℕ → is-zero-ℕ x
is-zero-leq-zero-ℕ zero-ℕ star = refl

is-zero-leq-zero-ℕ' :
  (x : ℕ) → x ≤-ℕ zero-ℕ → is-zero-ℕ' x
is-zero-leq-zero-ℕ' zero-ℕ star = refl

succ-leq-ℕ : (n : ℕ) → n ≤-ℕ (succ-ℕ n)
succ-leq-ℕ zero-ℕ = star
succ-leq-ℕ (succ-ℕ n) = succ-leq-ℕ n

concatenate-eq-leq-eq-ℕ :
  {x' x y y' : ℕ} → Id x' x → x ≤-ℕ y → Id y y' → x' ≤-ℕ y'
concatenate-eq-leq-eq-ℕ refl H refl = H

concatenate-leq-eq-ℕ :
  (m : ℕ) {n n' : ℕ} → m ≤-ℕ n → Id n n' → m ≤-ℕ n'
concatenate-leq-eq-ℕ m H refl = H

concatenate-eq-leq-ℕ :
  {m m' : ℕ} (n : ℕ) → Id m' m → m ≤-ℕ n → m' ≤-ℕ n
concatenate-eq-leq-ℕ n refl H = H

decide-leq-succ-ℕ :
  (m n : ℕ) → m ≤-ℕ (succ-ℕ n) → coprod (m ≤-ℕ n) (Id m (succ-ℕ n))
decide-leq-succ-ℕ zero-ℕ zero-ℕ l = inl star
decide-leq-succ-ℕ zero-ℕ (succ-ℕ n) l = inl star
decide-leq-succ-ℕ (succ-ℕ m) zero-ℕ l =
  inr (ap succ-ℕ (is-zero-leq-zero-ℕ m l))
decide-leq-succ-ℕ (succ-ℕ m) (succ-ℕ n) l =
  map-coprod id (ap succ-ℕ) (decide-leq-succ-ℕ m n l)

-- Exercise 6.3 (a)

refl-leq-ℕ : (n : ℕ) → n ≤-ℕ n
refl-leq-ℕ zero-ℕ = star
refl-leq-ℕ (succ-ℕ n) = refl-leq-ℕ n

leq-eq-ℕ : (m n : ℕ) → Id m n → m ≤-ℕ n
leq-eq-ℕ m .m refl = refl-leq-ℕ m

transitive-leq-ℕ :
  (n m l : ℕ) → (n ≤-ℕ m) → (m ≤-ℕ l) → (n ≤-ℕ l)
transitive-leq-ℕ zero-ℕ m l p q = star
transitive-leq-ℕ (succ-ℕ n) (succ-ℕ m) (succ-ℕ l) p q =
  transitive-leq-ℕ n m l p q

preserves-leq-succ-ℕ :
  (m n : ℕ) → m ≤-ℕ n → m ≤-ℕ (succ-ℕ n)
preserves-leq-succ-ℕ m n p = transitive-leq-ℕ m n (succ-ℕ n) p (succ-leq-ℕ n)

antisymmetric-leq-ℕ : (m n : ℕ) → m ≤-ℕ n → n ≤-ℕ m → Id m n
antisymmetric-leq-ℕ zero-ℕ zero-ℕ p q = refl
antisymmetric-leq-ℕ (succ-ℕ m) (succ-ℕ n) p q =
  ap succ-ℕ (antisymmetric-leq-ℕ m n p q)

-- Exercise 6.3 (b)

decide-leq-ℕ :
  (m n : ℕ) → coprod (m ≤-ℕ n) (n ≤-ℕ m)
decide-leq-ℕ zero-ℕ zero-ℕ = inl star
decide-leq-ℕ zero-ℕ (succ-ℕ n) = inl star
decide-leq-ℕ (succ-ℕ m) zero-ℕ = inr star
decide-leq-ℕ (succ-ℕ m) (succ-ℕ n) = decide-leq-ℕ m n

-- Exercise 6.3 (c)

preserves-order-add-ℕ :
  (k m n : ℕ) → m ≤-ℕ n → (add-ℕ m k) ≤-ℕ (add-ℕ n k)
preserves-order-add-ℕ zero-ℕ m n = id
preserves-order-add-ℕ (succ-ℕ k) m n = preserves-order-add-ℕ k m n

reflects-order-add-ℕ :
  (k m n : ℕ) → (add-ℕ m k) ≤-ℕ (add-ℕ n k) → m ≤-ℕ n
reflects-order-add-ℕ zero-ℕ m n = id
reflects-order-add-ℕ (succ-ℕ k) m n = reflects-order-add-ℕ k m n

-- Exercise 6.3 (d)

preserves-order-mul-ℕ :
  (k m n : ℕ) → m ≤-ℕ n → (mul-ℕ m k) ≤-ℕ (mul-ℕ n k)
preserves-order-mul-ℕ k zero-ℕ n p = star
preserves-order-mul-ℕ k (succ-ℕ m) (succ-ℕ n) p =
  preserves-order-add-ℕ k
    ( mul-ℕ m k)
    ( mul-ℕ n k)
    ( preserves-order-mul-ℕ k m n p)

preserves-order-mul-ℕ' :
  (k m n : ℕ) → m ≤-ℕ n → (mul-ℕ k m) ≤-ℕ (mul-ℕ k n)
preserves-order-mul-ℕ' k m n H =
  concatenate-eq-leq-eq-ℕ
    ( commutative-mul-ℕ k m)
    ( preserves-order-mul-ℕ k m n H)
    ( commutative-mul-ℕ n k)

reflects-order-mul-ℕ :
  (k m n : ℕ) → (mul-ℕ m (succ-ℕ k)) ≤-ℕ (mul-ℕ n (succ-ℕ k)) → m ≤-ℕ n
reflects-order-mul-ℕ k zero-ℕ n p = star
reflects-order-mul-ℕ k (succ-ℕ m) (succ-ℕ n) p =
  reflects-order-mul-ℕ k m n
    ( reflects-order-add-ℕ
      ( succ-ℕ k)
      ( mul-ℕ m (succ-ℕ k))
      ( mul-ℕ n (succ-ℕ k))
      ( p))

-- We also record the fact that x ≤-ℕ mul-ℕ x (succ-ℕ k)

leq-mul-ℕ :
  (k x : ℕ) → x ≤-ℕ (mul-ℕ x (succ-ℕ k))
leq-mul-ℕ k x =
  concatenate-eq-leq-ℕ
    ( mul-ℕ x (succ-ℕ k))
    ( inv (right-unit-law-mul-ℕ x))
    ( preserves-order-mul-ℕ' x one-ℕ (succ-ℕ k) (leq-zero-ℕ k))

leq-mul-ℕ' :
  (k x : ℕ) → x ≤-ℕ (mul-ℕ (succ-ℕ k) x)
leq-mul-ℕ' k x =
  concatenate-leq-eq-ℕ x
    ( leq-mul-ℕ k x)
    ( commutative-mul-ℕ x (succ-ℕ k))

leq-mul-is-nonzero-ℕ :
  (k x : ℕ) → is-nonzero-ℕ k → x ≤-ℕ (mul-ℕ x k)
leq-mul-is-nonzero-ℕ k x H with is-successor-is-nonzero-ℕ H
... | pair l refl = leq-mul-ℕ l x

leq-mul-is-nonzero-ℕ' :
  (k x : ℕ) → is-nonzero-ℕ k → x ≤-ℕ (mul-ℕ k x)
leq-mul-is-nonzero-ℕ' k x H with is-successor-is-nonzero-ℕ H
... | pair l refl = leq-mul-ℕ' l x

-- Exercise 6.3 (e)

leq-min-ℕ :
  (k m n : ℕ) → k ≤-ℕ m → k ≤-ℕ n → k ≤-ℕ (min-ℕ m n)
leq-min-ℕ zero-ℕ zero-ℕ zero-ℕ H K = star
leq-min-ℕ zero-ℕ zero-ℕ (succ-ℕ n) H K = star
leq-min-ℕ zero-ℕ (succ-ℕ m) zero-ℕ H K = star
leq-min-ℕ zero-ℕ (succ-ℕ m) (succ-ℕ n) H K = star
leq-min-ℕ (succ-ℕ k) (succ-ℕ m) (succ-ℕ n) H K = leq-min-ℕ k m n H K

leq-left-leq-min-ℕ :
  (k m n : ℕ) → k ≤-ℕ (min-ℕ m n) → k ≤-ℕ m
leq-left-leq-min-ℕ zero-ℕ zero-ℕ zero-ℕ H = star
leq-left-leq-min-ℕ zero-ℕ zero-ℕ (succ-ℕ n) H = star
leq-left-leq-min-ℕ zero-ℕ (succ-ℕ m) zero-ℕ H = star
leq-left-leq-min-ℕ zero-ℕ (succ-ℕ m) (succ-ℕ n) H = star
leq-left-leq-min-ℕ (succ-ℕ k) (succ-ℕ m) (succ-ℕ n) H =
  leq-left-leq-min-ℕ k m n H

leq-right-leq-min-ℕ :
  (k m n : ℕ) → k ≤-ℕ (min-ℕ m n) → k ≤-ℕ n
leq-right-leq-min-ℕ zero-ℕ zero-ℕ zero-ℕ H = star
leq-right-leq-min-ℕ zero-ℕ zero-ℕ (succ-ℕ n) H = star
leq-right-leq-min-ℕ zero-ℕ (succ-ℕ m) zero-ℕ H = star
leq-right-leq-min-ℕ zero-ℕ (succ-ℕ m) (succ-ℕ n) H = star
leq-right-leq-min-ℕ (succ-ℕ k) (succ-ℕ m) (succ-ℕ n) H =
  leq-right-leq-min-ℕ k m n H

leq-max-ℕ :
  (k m n : ℕ) → m ≤-ℕ k → n ≤-ℕ k → (max-ℕ m n) ≤-ℕ k
leq-max-ℕ zero-ℕ zero-ℕ zero-ℕ H K = star
leq-max-ℕ (succ-ℕ k) zero-ℕ zero-ℕ H K = star
leq-max-ℕ (succ-ℕ k) zero-ℕ (succ-ℕ n) H K = K
leq-max-ℕ (succ-ℕ k) (succ-ℕ m) zero-ℕ H K = H
leq-max-ℕ (succ-ℕ k) (succ-ℕ m) (succ-ℕ n) H K = leq-max-ℕ k m n H K

leq-left-leq-max-ℕ :
  (k m n : ℕ) → (max-ℕ m n) ≤-ℕ k → m ≤-ℕ k
leq-left-leq-max-ℕ k zero-ℕ zero-ℕ H = star
leq-left-leq-max-ℕ k zero-ℕ (succ-ℕ n) H = star
leq-left-leq-max-ℕ k (succ-ℕ m) zero-ℕ H = H
leq-left-leq-max-ℕ (succ-ℕ k) (succ-ℕ m) (succ-ℕ n) H =
  leq-left-leq-max-ℕ k m n H

leq-right-leq-max-ℕ :
  (k m n : ℕ) → (max-ℕ m n) ≤-ℕ k → n ≤-ℕ k
leq-right-leq-max-ℕ k zero-ℕ zero-ℕ H = star
leq-right-leq-max-ℕ k zero-ℕ (succ-ℕ n) H = H
leq-right-leq-max-ℕ k (succ-ℕ m) zero-ℕ H = star
leq-right-leq-max-ℕ (succ-ℕ k) (succ-ℕ m) (succ-ℕ n) H =
  leq-right-leq-max-ℕ k m n H

-- Exercise 6.4

-- The definition of <

le-ℕ : ℕ → ℕ → UU lzero
le-ℕ m zero-ℕ = empty
le-ℕ zero-ℕ (succ-ℕ m) = unit
le-ℕ (succ-ℕ n) (succ-ℕ m) = le-ℕ n m

_<_ = le-ℕ

anti-reflexive-le-ℕ : (n : ℕ) → ¬ (n < n)
anti-reflexive-le-ℕ zero-ℕ = ind-empty
anti-reflexive-le-ℕ (succ-ℕ n) = anti-reflexive-le-ℕ n

transitive-le-ℕ : (n m l : ℕ) → (le-ℕ n m) → (le-ℕ m l) → (le-ℕ n l)
transitive-le-ℕ zero-ℕ (succ-ℕ m) (succ-ℕ l) p q = star
transitive-le-ℕ (succ-ℕ n) (succ-ℕ m) (succ-ℕ l) p q =
  transitive-le-ℕ n m l p q

succ-le-ℕ : (n : ℕ) → le-ℕ n (succ-ℕ n)
succ-le-ℕ zero-ℕ = star
succ-le-ℕ (succ-ℕ n) = succ-le-ℕ n

preserves-le-succ-ℕ :
  (m n : ℕ) → le-ℕ m n → le-ℕ m (succ-ℕ n)
preserves-le-succ-ℕ m n H =
  transitive-le-ℕ m n (succ-ℕ n) H (succ-le-ℕ n)

anti-symmetric-le-ℕ : (m n : ℕ) → le-ℕ m n → le-ℕ n m → Id m n
anti-symmetric-le-ℕ (succ-ℕ m) (succ-ℕ n) p q =
  ap succ-ℕ (anti-symmetric-le-ℕ m n p q)

contradiction-le-ℕ : (m n : ℕ) → le-ℕ m n → ¬ (n ≤-ℕ m)
contradiction-le-ℕ zero-ℕ (succ-ℕ n) H K = K
contradiction-le-ℕ (succ-ℕ m) (succ-ℕ n) H = contradiction-le-ℕ m n H

contradiction-le-ℕ' : (m n : ℕ) → n ≤-ℕ m → ¬ (le-ℕ m n)
contradiction-le-ℕ' m n K H = contradiction-le-ℕ m n H K

leq-not-le-ℕ : (m n : ℕ) → ¬ (le-ℕ m n) → n ≤-ℕ m
leq-not-le-ℕ zero-ℕ zero-ℕ H = star
leq-not-le-ℕ zero-ℕ (succ-ℕ n) H = ex-falso (H star)
leq-not-le-ℕ (succ-ℕ m) zero-ℕ H = star
leq-not-le-ℕ (succ-ℕ m) (succ-ℕ n) H = leq-not-le-ℕ m n H

is-nonzero-le-ℕ : (m n : ℕ) → le-ℕ m n → is-nonzero-ℕ n
is-nonzero-le-ℕ m n H p = tr (le-ℕ m) p H

contradiction-leq-ℕ : (m n : ℕ) → m ≤-ℕ n → ¬ ((succ-ℕ n) ≤-ℕ m)
contradiction-leq-ℕ (succ-ℕ m) (succ-ℕ n) H K = contradiction-leq-ℕ m n H K

contradiction-leq-ℕ' : (m n : ℕ) → (succ-ℕ n) ≤-ℕ m → ¬ (m ≤-ℕ n)
contradiction-leq-ℕ' m n K H = contradiction-leq-ℕ m n H K

leq-le-ℕ :
  {x y : ℕ} → le-ℕ x y → x ≤-ℕ y
leq-le-ℕ {zero-ℕ} {succ-ℕ y} H = star
leq-le-ℕ {succ-ℕ x} {succ-ℕ y} H = leq-le-ℕ {x} {y} H

concatenate-leq-le-ℕ :
  {x y z : ℕ} → x ≤-ℕ y → le-ℕ y z → le-ℕ x z
concatenate-leq-le-ℕ {zero-ℕ} {zero-ℕ} {succ-ℕ z} H K = star
concatenate-leq-le-ℕ {zero-ℕ} {succ-ℕ y} {succ-ℕ z} H K = star
concatenate-leq-le-ℕ {succ-ℕ x} {succ-ℕ y} {succ-ℕ z} H K =
  concatenate-leq-le-ℕ {x} {y} {z} H K

concatenate-le-leq-ℕ :
  {x y z : ℕ} → le-ℕ x y → y ≤-ℕ z → le-ℕ x z
concatenate-le-leq-ℕ {zero-ℕ} {succ-ℕ y} {succ-ℕ z} H K = star
concatenate-le-leq-ℕ {succ-ℕ x} {succ-ℕ y} {succ-ℕ z} H K =
  concatenate-le-leq-ℕ {x} {y} {z} H K

concatenate-eq-le-eq-ℕ :
  {x y z w : ℕ} → Id x y → le-ℕ y z → Id z w → le-ℕ x w
concatenate-eq-le-eq-ℕ refl p refl = p

concatenate-eq-le-ℕ :
  {x y z : ℕ} → Id x y → le-ℕ y z → le-ℕ x z
concatenate-eq-le-ℕ refl p = p

concatenate-le-eq-ℕ :
  {x y z : ℕ} → le-ℕ x y → Id y z → le-ℕ x z
concatenate-le-eq-ℕ p refl = p

le-succ-ℕ : {x : ℕ} → le-ℕ x (succ-ℕ x)
le-succ-ℕ {zero-ℕ} = star
le-succ-ℕ {succ-ℕ x} = le-succ-ℕ {x}

le-leq-neq-ℕ : {x y : ℕ} → x ≤-ℕ y → ¬ (Id x y) → le-ℕ x y
le-leq-neq-ℕ {zero-ℕ} {zero-ℕ} l f = ex-falso (f refl)
le-leq-neq-ℕ {zero-ℕ} {succ-ℕ y} l f = star
le-leq-neq-ℕ {succ-ℕ x} {succ-ℕ y} l f =
  le-leq-neq-ℕ {x} {y} l (λ p → f (ap succ-ℕ p))

linear-le-ℕ : (x y : ℕ) → coprod (le-ℕ x y) (coprod (Id x y) (le-ℕ y x))
linear-le-ℕ zero-ℕ zero-ℕ = inr (inl refl)
linear-le-ℕ zero-ℕ (succ-ℕ y) = inl star
linear-le-ℕ (succ-ℕ x) zero-ℕ = inr (inr star)
linear-le-ℕ (succ-ℕ x) (succ-ℕ y) =
  map-coprod id (map-coprod (ap succ-ℕ) id) (linear-le-ℕ x y)

-- Exercise 6.5

-- Exercise 6.5 (a)

-- We define a distance function on ℕ --

dist-ℕ : ℕ → ℕ → ℕ
dist-ℕ zero-ℕ n = n
dist-ℕ (succ-ℕ m) zero-ℕ = succ-ℕ m
dist-ℕ (succ-ℕ m) (succ-ℕ n) = dist-ℕ m n

dist-ℕ' : ℕ → ℕ → ℕ
dist-ℕ' m n = dist-ℕ n m

ap-dist-ℕ :
  {m n m' n' : ℕ} → Id m m' → Id n n' → Id (dist-ℕ m n) (dist-ℕ m' n')
ap-dist-ℕ p q = ap-binary dist-ℕ p q

{- We show that two natural numbers are equal if and only if their distance is
   zero. -}

eq-dist-ℕ : (m n : ℕ) → is-zero-ℕ (dist-ℕ m n) → Id m n
eq-dist-ℕ zero-ℕ zero-ℕ p = refl
eq-dist-ℕ (succ-ℕ m) (succ-ℕ n) p = ap succ-ℕ (eq-dist-ℕ m n p)

dist-eq-ℕ' : (n : ℕ) → is-zero-ℕ (dist-ℕ n n)
dist-eq-ℕ' zero-ℕ = refl
dist-eq-ℕ' (succ-ℕ n) = dist-eq-ℕ' n

dist-eq-ℕ : (m n : ℕ) → Id m n → is-zero-ℕ (dist-ℕ m n)
dist-eq-ℕ m .m refl = dist-eq-ℕ' m

is-one-dist-succ-ℕ : (x : ℕ) → is-one-ℕ (dist-ℕ x (succ-ℕ x))
is-one-dist-succ-ℕ zero-ℕ = refl
is-one-dist-succ-ℕ (succ-ℕ x) = is-one-dist-succ-ℕ x

is-one-dist-succ-ℕ' : (x : ℕ) → is-one-ℕ (dist-ℕ (succ-ℕ x) x)
is-one-dist-succ-ℕ' zero-ℕ = refl
is-one-dist-succ-ℕ' (succ-ℕ x) = is-one-dist-succ-ℕ' x

-- The distance function is symmetric --

symmetric-dist-ℕ :
  (m n : ℕ) → Id (dist-ℕ m n) (dist-ℕ n m)
symmetric-dist-ℕ zero-ℕ zero-ℕ = refl
symmetric-dist-ℕ zero-ℕ (succ-ℕ n) = refl
symmetric-dist-ℕ (succ-ℕ m) zero-ℕ = refl
symmetric-dist-ℕ (succ-ℕ m) (succ-ℕ n) = symmetric-dist-ℕ m n

-- We compute the distance from zero --

left-unit-law-dist-ℕ :
  (n : ℕ) → Id (dist-ℕ zero-ℕ n) n
left-unit-law-dist-ℕ zero-ℕ = refl
left-unit-law-dist-ℕ (succ-ℕ n) = refl

right-unit-law-dist-ℕ :
  (n : ℕ) → Id (dist-ℕ n zero-ℕ) n
right-unit-law-dist-ℕ zero-ℕ = refl
right-unit-law-dist-ℕ (succ-ℕ n) = refl

-- We prove the triangle inequality --

triangle-inequality-dist-ℕ :
  (m n k : ℕ) → (dist-ℕ m n) ≤-ℕ (add-ℕ (dist-ℕ m k) (dist-ℕ k n))
triangle-inequality-dist-ℕ zero-ℕ zero-ℕ zero-ℕ = star
triangle-inequality-dist-ℕ zero-ℕ zero-ℕ (succ-ℕ k) = star
triangle-inequality-dist-ℕ zero-ℕ (succ-ℕ n) zero-ℕ =
  tr ( leq-ℕ (succ-ℕ n))
     ( inv (left-unit-law-add-ℕ (succ-ℕ n)))
     ( refl-leq-ℕ (succ-ℕ n))
triangle-inequality-dist-ℕ zero-ℕ (succ-ℕ n) (succ-ℕ k) =
  concatenate-eq-leq-eq-ℕ
    ( inv (ap succ-ℕ (left-unit-law-dist-ℕ n)))
    ( triangle-inequality-dist-ℕ zero-ℕ n k)
    ( ( ap (succ-ℕ ∘ (add-ℕ' (dist-ℕ k n))) (left-unit-law-dist-ℕ k)) ∙
      ( inv (left-successor-law-add-ℕ k (dist-ℕ k n))))
triangle-inequality-dist-ℕ (succ-ℕ m) zero-ℕ zero-ℕ = refl-leq-ℕ (succ-ℕ m)
triangle-inequality-dist-ℕ (succ-ℕ m) zero-ℕ (succ-ℕ k) =
  concatenate-eq-leq-eq-ℕ
    ( inv (ap succ-ℕ (right-unit-law-dist-ℕ m)))
    ( triangle-inequality-dist-ℕ m zero-ℕ k)
    ( ap (succ-ℕ ∘ (add-ℕ (dist-ℕ m k))) (right-unit-law-dist-ℕ k))
triangle-inequality-dist-ℕ (succ-ℕ m) (succ-ℕ n) zero-ℕ =
  concatenate-leq-eq-ℕ
    ( dist-ℕ m n)
    ( transitive-leq-ℕ
      ( dist-ℕ m n)
      ( succ-ℕ (add-ℕ (dist-ℕ m zero-ℕ) (dist-ℕ zero-ℕ n)))
      ( succ-ℕ (succ-ℕ (add-ℕ (dist-ℕ m zero-ℕ) (dist-ℕ zero-ℕ n)))) 
      ( transitive-leq-ℕ
        ( dist-ℕ m n)
        ( add-ℕ (dist-ℕ m zero-ℕ) (dist-ℕ zero-ℕ n))
        ( succ-ℕ (add-ℕ (dist-ℕ m zero-ℕ) (dist-ℕ zero-ℕ n)))
        ( triangle-inequality-dist-ℕ m n zero-ℕ)
        ( succ-leq-ℕ (add-ℕ (dist-ℕ m zero-ℕ) (dist-ℕ zero-ℕ n))))
      ( succ-leq-ℕ (succ-ℕ (add-ℕ (dist-ℕ m zero-ℕ) (dist-ℕ zero-ℕ n)))))
    ( ( ap (succ-ℕ ∘ succ-ℕ)
           ( ap-add-ℕ (right-unit-law-dist-ℕ m) (left-unit-law-dist-ℕ n))) ∙
      ( inv (left-successor-law-add-ℕ m (succ-ℕ n))))
triangle-inequality-dist-ℕ (succ-ℕ m) (succ-ℕ n) (succ-ℕ k) =
  triangle-inequality-dist-ℕ m n k

-- Exercise 6.5 (b)

-- We show that dist-ℕ x y is a solution to a simple equation.

is-additive-right-inverse-dist-ℕ :
  (x y : ℕ) → x ≤-ℕ y → Id (add-ℕ x (dist-ℕ x y)) y
is-additive-right-inverse-dist-ℕ zero-ℕ zero-ℕ H = refl
is-additive-right-inverse-dist-ℕ zero-ℕ (succ-ℕ y) star = left-unit-law-add-ℕ (succ-ℕ y)
is-additive-right-inverse-dist-ℕ (succ-ℕ x) (succ-ℕ y) H =
  ( left-successor-law-add-ℕ x (dist-ℕ x y)) ∙
  ( ap succ-ℕ (is-additive-right-inverse-dist-ℕ x y H))

-- If three elements are ordered linearly, then their distances add up.

triangle-equality-dist-ℕ :
  (x y z : ℕ) → (x ≤-ℕ y) → (y ≤-ℕ z) →
  Id (add-ℕ (dist-ℕ x y) (dist-ℕ y z)) (dist-ℕ x z)
triangle-equality-dist-ℕ zero-ℕ zero-ℕ zero-ℕ H1 H2 = refl
triangle-equality-dist-ℕ zero-ℕ zero-ℕ (succ-ℕ z) star star =
  ap succ-ℕ (left-unit-law-add-ℕ z)
triangle-equality-dist-ℕ zero-ℕ (succ-ℕ y) (succ-ℕ z) star H2 =
  left-successor-law-add-ℕ y (dist-ℕ y z) ∙
  ap succ-ℕ (is-additive-right-inverse-dist-ℕ y z H2)
triangle-equality-dist-ℕ (succ-ℕ x) (succ-ℕ y) (succ-ℕ z) H1 H2 =
  triangle-equality-dist-ℕ x y z H1 H2

rewrite-left-add-dist-ℕ :
  (x y z : ℕ) → Id (add-ℕ x y) z → Id x (dist-ℕ y z)
rewrite-left-add-dist-ℕ zero-ℕ zero-ℕ .zero-ℕ refl = refl
rewrite-left-add-dist-ℕ zero-ℕ (succ-ℕ y) .(succ-ℕ (add-ℕ zero-ℕ y)) refl =
  ( inv (dist-eq-ℕ' y)) ∙
  ( inv (ap (dist-ℕ (succ-ℕ y)) (left-unit-law-add-ℕ (succ-ℕ y))))
rewrite-left-add-dist-ℕ (succ-ℕ x) zero-ℕ .(succ-ℕ x) refl = refl
rewrite-left-add-dist-ℕ
  (succ-ℕ x) (succ-ℕ y) .(succ-ℕ (add-ℕ (succ-ℕ x) y)) refl =
  rewrite-left-add-dist-ℕ (succ-ℕ x) y (add-ℕ (succ-ℕ x) y) refl

rewrite-left-dist-add-ℕ :
  (x y z : ℕ) → y ≤-ℕ z → Id x (dist-ℕ y z) → Id (add-ℕ x y) z
rewrite-left-dist-add-ℕ .(dist-ℕ y z) y z H refl =
  ( commutative-add-ℕ (dist-ℕ y z) y) ∙
  ( is-additive-right-inverse-dist-ℕ y z H)

rewrite-right-add-dist-ℕ :
  (x y z : ℕ) → Id (add-ℕ x y) z → Id y (dist-ℕ x z)
rewrite-right-add-dist-ℕ x y z p =
  rewrite-left-add-dist-ℕ y x z (commutative-add-ℕ y x ∙ p)

rewrite-right-dist-add-ℕ :
  (x y z : ℕ) → x ≤-ℕ z → Id y (dist-ℕ x z) → Id (add-ℕ x y) z
rewrite-right-dist-add-ℕ x .(dist-ℕ x z) z H refl =
  is-additive-right-inverse-dist-ℕ x z H

leq-dist-ℕ :
  (x y : ℕ) → x ≤-ℕ y → dist-ℕ x y ≤-ℕ y
leq-dist-ℕ zero-ℕ zero-ℕ H = refl-leq-ℕ zero-ℕ
leq-dist-ℕ zero-ℕ (succ-ℕ y) H = refl-leq-ℕ y
leq-dist-ℕ (succ-ℕ x) (succ-ℕ y) H =
  transitive-leq-ℕ (dist-ℕ x y) y (succ-ℕ y) (leq-dist-ℕ x y H) (succ-leq-ℕ y)

-- We show that dist-ℕ is translation invariant

translation-invariant-dist-ℕ :
  (k m n : ℕ) → Id (dist-ℕ (add-ℕ k m) (add-ℕ k n)) (dist-ℕ m n)
translation-invariant-dist-ℕ zero-ℕ m n =
  ap-dist-ℕ (left-unit-law-add-ℕ m) (left-unit-law-add-ℕ n)
translation-invariant-dist-ℕ (succ-ℕ k)  m n =
  ( ap-dist-ℕ (left-successor-law-add-ℕ k m) (left-successor-law-add-ℕ k n)) ∙
  ( translation-invariant-dist-ℕ k m n)

translation-invariant-dist-ℕ' :
  (k m n : ℕ) → Id (dist-ℕ (add-ℕ m k) (add-ℕ n k)) (dist-ℕ m n)
translation-invariant-dist-ℕ' k m n =
  ( ap-dist-ℕ (commutative-add-ℕ m k) (commutative-add-ℕ n k)) ∙
  ( translation-invariant-dist-ℕ k m n)

-- We show that dist-ℕ is linear with respect to scalar multiplication

left-distributive-mul-dist-ℕ :
  (m n k : ℕ) → Id (mul-ℕ k (dist-ℕ m n)) (dist-ℕ (mul-ℕ k m) (mul-ℕ k n))
left-distributive-mul-dist-ℕ zero-ℕ zero-ℕ zero-ℕ = refl
left-distributive-mul-dist-ℕ zero-ℕ zero-ℕ (succ-ℕ k) = left-distributive-mul-dist-ℕ zero-ℕ zero-ℕ k
left-distributive-mul-dist-ℕ zero-ℕ (succ-ℕ n) zero-ℕ = refl
left-distributive-mul-dist-ℕ zero-ℕ (succ-ℕ n) (succ-ℕ k) =
  ap ( dist-ℕ' (mul-ℕ (succ-ℕ k) (succ-ℕ n)))
     ( inv (right-zero-law-mul-ℕ (succ-ℕ k)))
left-distributive-mul-dist-ℕ (succ-ℕ m) zero-ℕ zero-ℕ = refl
left-distributive-mul-dist-ℕ (succ-ℕ m) zero-ℕ (succ-ℕ k) =
  ap ( dist-ℕ (mul-ℕ (succ-ℕ k) (succ-ℕ m)))
     ( inv (right-zero-law-mul-ℕ (succ-ℕ k)))
left-distributive-mul-dist-ℕ (succ-ℕ m) (succ-ℕ n) zero-ℕ = refl
left-distributive-mul-dist-ℕ (succ-ℕ m) (succ-ℕ n) (succ-ℕ k) =
  inv
    ( ( ap-dist-ℕ
        ( right-successor-law-mul-ℕ (succ-ℕ k) m)
        ( right-successor-law-mul-ℕ (succ-ℕ k) n)) ∙
      ( ( translation-invariant-dist-ℕ
          ( succ-ℕ k)
          ( mul-ℕ (succ-ℕ k) m)
          ( mul-ℕ (succ-ℕ k) n)) ∙
        ( inv (left-distributive-mul-dist-ℕ m n (succ-ℕ k)))))

right-distributive-mul-dist-ℕ :
  (x y k : ℕ) → Id (mul-ℕ (dist-ℕ x y) k) (dist-ℕ (mul-ℕ x k) (mul-ℕ y k))
right-distributive-mul-dist-ℕ x y k =
  ( commutative-mul-ℕ (dist-ℕ x y) k) ∙
  ( ( left-distributive-mul-dist-ℕ x y k) ∙
    ( ap-dist-ℕ (commutative-mul-ℕ k x) (commutative-mul-ℕ k y)))

-- Exercise 6.5 (d)

is-difference-dist-ℕ :
  (x y : ℕ) → x ≤-ℕ y → Id (add-ℕ x (dist-ℕ x y)) y
is-difference-dist-ℕ zero-ℕ zero-ℕ H = refl
is-difference-dist-ℕ zero-ℕ (succ-ℕ y) H = left-unit-law-add-ℕ (succ-ℕ y)
is-difference-dist-ℕ (succ-ℕ x) (succ-ℕ y) H =
  ( left-successor-law-add-ℕ x (dist-ℕ x y)) ∙
  ( ap succ-ℕ (is-difference-dist-ℕ x y H))

is-difference-dist-ℕ' :
  (x y : ℕ) → x ≤-ℕ y → Id (add-ℕ (dist-ℕ x y) x) y
is-difference-dist-ℕ' x y H =
  ( commutative-add-ℕ (dist-ℕ x y) x) ∙
  ( is-difference-dist-ℕ x y H)

--------------------------------------------------------------------------------

-- Exercise 6.5

is-zero-ℤ : ℤ → UU lzero
is-zero-ℤ x = Id x zero-ℤ

is-nonzero-ℤ : ℤ → UU lzero
is-nonzero-ℤ k = ¬ (is-zero-ℤ k)

is-one-ℤ : ℤ → UU lzero
is-one-ℤ x = Id x one-ℤ

is-neg-one-ℤ : ℤ → UU lzero
is-neg-one-ℤ x = Id x neg-one-ℤ

-- We introduce the absolute value of an integer. --

abs-ℤ : ℤ → ℕ
abs-ℤ (inl x) = succ-ℕ x
abs-ℤ (inr (inl star)) = zero-ℕ
abs-ℤ (inr (inr x)) = succ-ℕ x

int-abs-ℤ : ℤ → ℤ
int-abs-ℤ = int-ℕ ∘ abs-ℤ

abs-int-ℕ : (x : ℕ) → Id (abs-ℤ (int-ℕ x)) x
abs-int-ℕ zero-ℕ = refl
abs-int-ℕ (succ-ℕ x) = refl

abs-neg-ℤ : (x : ℤ) → Id (abs-ℤ (neg-ℤ x)) (abs-ℤ x)
abs-neg-ℤ (inl x) = refl
abs-neg-ℤ (inr (inl star)) = refl
abs-neg-ℤ (inr (inr x)) = refl

is-injective-int-ℕ : is-injective int-ℕ
is-injective-int-ℕ {zero-ℕ} {zero-ℕ} p = refl
is-injective-int-ℕ {succ-ℕ x} {succ-ℕ y} p =
  eq-Eq-ℕ (succ-ℕ x) (succ-ℕ y) (Eq-eq-ℤ p)

is-nonzero-int-ℕ : (n : ℕ) → is-nonzero-ℕ n → is-nonzero-ℤ (int-ℕ n)
is-nonzero-int-ℕ zero-ℕ H p = H refl

eq-abs-ℤ : (x : ℤ) → is-zero-ℕ (abs-ℤ x) → is-zero-ℤ x
eq-abs-ℤ (inl x) p = ex-falso (Peano-8 x p)
eq-abs-ℤ (inr (inl star)) p = refl
eq-abs-ℤ (inr (inr x)) p = ex-falso (Peano-8 x p)

abs-eq-ℤ : (x : ℤ) → is-zero-ℤ x → is-zero-ℕ (abs-ℤ x)
abs-eq-ℤ .zero-ℤ refl = refl

predecessor-law-abs-ℤ :
  (x : ℤ) → (abs-ℤ (pred-ℤ x)) ≤-ℕ (succ-ℕ (abs-ℤ x))
predecessor-law-abs-ℤ (inl x) =
  refl-leq-ℕ (succ-ℕ x)
predecessor-law-abs-ℤ (inr (inl star)) =
  refl-leq-ℕ zero-ℕ
predecessor-law-abs-ℤ (inr (inr zero-ℕ)) =
  star
predecessor-law-abs-ℤ (inr (inr (succ-ℕ x))) =
  preserves-leq-succ-ℕ x (succ-ℕ x) (succ-leq-ℕ x)

successor-law-abs-ℤ :
  (x : ℤ) → (abs-ℤ (succ-ℤ x)) ≤-ℕ (succ-ℕ (abs-ℤ x))
successor-law-abs-ℤ (inl zero-ℕ) =
  star
successor-law-abs-ℤ (inl (succ-ℕ x)) =
  preserves-leq-succ-ℕ x (succ-ℕ x) (succ-leq-ℕ x)
successor-law-abs-ℤ (inr (inl star)) =
  refl-leq-ℕ zero-ℕ
successor-law-abs-ℤ (inr (inr x)) =
  refl-leq-ℕ (succ-ℕ x)

subadditive-abs-ℤ :
  (x y : ℤ) → (abs-ℤ (add-ℤ x y)) ≤-ℕ (add-ℕ (abs-ℤ x) (abs-ℤ y))
subadditive-abs-ℤ x (inl zero-ℕ) =
  concatenate-eq-leq-eq-ℕ
    ( ap abs-ℤ (add-neg-one-right-ℤ x))
    ( predecessor-law-abs-ℤ x)
    ( refl)
subadditive-abs-ℤ x (inl (succ-ℕ y)) =
  concatenate-eq-leq-eq-ℕ
    ( ap abs-ℤ (right-predecessor-law-add-ℤ x (inl y)))
    ( transitive-leq-ℕ
      ( abs-ℤ (pred-ℤ (add-ℤ x (inl y))))
      ( succ-ℕ (abs-ℤ (add-ℤ x (inl y))))
      ( add-ℕ (abs-ℤ x) (succ-ℕ (succ-ℕ y)))
      ( predecessor-law-abs-ℤ (add-ℤ x (inl y)))
      ( subadditive-abs-ℤ x (inl y)))
    ( refl)
subadditive-abs-ℤ x (inr (inl star)) =
  concatenate-eq-leq-eq-ℕ
    ( ap abs-ℤ (right-unit-law-add-ℤ x))
    ( refl-leq-ℕ (abs-ℤ x))
    ( refl)
subadditive-abs-ℤ x (inr (inr zero-ℕ)) =
  concatenate-eq-leq-eq-ℕ
    ( ap abs-ℤ (add-one-right-ℤ x))
    ( successor-law-abs-ℤ x)
    ( refl)
subadditive-abs-ℤ x (inr (inr (succ-ℕ y))) =
  concatenate-eq-leq-eq-ℕ
    ( ap abs-ℤ (right-successor-law-add-ℤ x (inr (inr y))))
    ( transitive-leq-ℕ
      ( abs-ℤ (succ-ℤ (add-ℤ x (inr (inr y)))))
      ( succ-ℕ (abs-ℤ (add-ℤ x (inr (inr y)))))
      ( succ-ℕ (add-ℕ (abs-ℤ x) (succ-ℕ y)))
      ( successor-law-abs-ℤ (add-ℤ x (inr (inr y))))
      ( subadditive-abs-ℤ x (inr (inr y))))
    ( refl)

negative-law-abs-ℤ :
  (x : ℤ) → Id (abs-ℤ (neg-ℤ x)) (abs-ℤ x)
negative-law-abs-ℤ (inl x) = refl
negative-law-abs-ℤ (inr (inl star)) = refl
negative-law-abs-ℤ (inr (inr x)) = refl

--------------------------------------------------------------------------------


-- Exercise 6.6

{- In this exercise we were asked to define the relations ≤-ℕ and < on the 
   integers. As a criterion of correctness, we were then also asked to show 
   that the type of all integers l satisfying k ≤-ℕ l satisfy the induction 
   principle of the natural numbers. -}

-- We introduce nonnegative integers

is-nonnegative-ℤ : ℤ → UU lzero
is-nonnegative-ℤ (inl x) = empty
is-nonnegative-ℤ (inr k) = unit

is-nonnegative-eq-ℤ :
  {x y : ℤ} → Id x y → is-nonnegative-ℤ x → is-nonnegative-ℤ y
is-nonnegative-eq-ℤ refl = id

is-zero-is-nonnegative-ℤ :
  {x : ℤ} → is-nonnegative-ℤ x → is-nonnegative-ℤ (neg-ℤ x) → is-zero-ℤ x
is-zero-is-nonnegative-ℤ {inr (inl star)} H K = refl

is-nonnegative-succ-ℤ :
  (k : ℤ) → is-nonnegative-ℤ k → is-nonnegative-ℤ (succ-ℤ k)
is-nonnegative-succ-ℤ (inr (inl star)) p = star
is-nonnegative-succ-ℤ (inr (inr x)) p = star

is-nonnegative-add-ℤ :
  (k l : ℤ) →
  is-nonnegative-ℤ k → is-nonnegative-ℤ l → is-nonnegative-ℤ (add-ℤ k l)
is-nonnegative-add-ℤ (inr (inl star)) (inr (inl star)) p q = star
is-nonnegative-add-ℤ (inr (inl star)) (inr (inr n)) p q = star
is-nonnegative-add-ℤ (inr (inr zero-ℕ)) (inr (inl star)) p q = star
is-nonnegative-add-ℤ (inr (inr (succ-ℕ n))) (inr (inl star)) star star =
  is-nonnegative-succ-ℤ
    ( add-ℤ (inr (inr n)) (inr (inl star)))
    ( is-nonnegative-add-ℤ (inr (inr n)) (inr (inl star)) star star)
is-nonnegative-add-ℤ (inr (inr zero-ℕ)) (inr (inr m)) star star = star
is-nonnegative-add-ℤ (inr (inr (succ-ℕ n))) (inr (inr m)) star star =
  is-nonnegative-succ-ℤ
    ( add-ℤ (inr (inr n)) (inr (inr m)))
    ( is-nonnegative-add-ℤ (inr (inr n)) (inr (inr m)) star star)

-- We introduce positive integers

is-positive-ℤ : ℤ → UU lzero
is-positive-ℤ (inl x) = empty
is-positive-ℤ (inr (inl x)) = empty
is-positive-ℤ (inr (inr x)) = unit

positive-ℤ : UU lzero
positive-ℤ = Σ ℤ is-positive-ℤ

is-nonnegative-is-positive-ℤ : {x : ℤ} → is-positive-ℤ x → is-nonnegative-ℤ x
is-nonnegative-is-positive-ℤ {inr (inr x)} H = H

is-nonzero-is-positive-ℤ : (x : ℤ) → is-positive-ℤ x → is-nonzero-ℤ x
is-nonzero-is-positive-ℤ (inr (inr x)) H p = Eq-eq-ℤ p

is-positive-eq-ℤ : {x y : ℤ} → Id x y → is-positive-ℤ x → is-positive-ℤ y
is-positive-eq-ℤ {x} refl = id

is-positive-one-ℤ : is-positive-ℤ one-ℤ
is-positive-one-ℤ = star

one-positive-ℤ : positive-ℤ
pr1 one-positive-ℤ = one-ℤ
pr2 one-positive-ℤ = is-positive-one-ℤ

is-positive-succ-ℤ : {x : ℤ} → is-nonnegative-ℤ x → is-positive-ℤ (succ-ℤ x)
is-positive-succ-ℤ {inr (inl star)} H = is-positive-one-ℤ
is-positive-succ-ℤ {inr (inr x)} H = star

is-positive-add-ℤ :
  {x y : ℤ} → is-positive-ℤ x → is-positive-ℤ y → is-positive-ℤ (add-ℤ x y)
is-positive-add-ℤ {inr (inr zero-ℕ)} {inr (inr y)} H K = star
is-positive-add-ℤ {inr (inr (succ-ℕ x))} {inr (inr y)} H K =
  is-positive-succ-ℤ
    ( is-nonnegative-is-positive-ℤ
      ( is-positive-add-ℤ {inr (inr x)} {inr (inr y)} star star))

is-positive-mul-ℤ :
  {x y : ℤ} → is-positive-ℤ x → is-positive-ℤ y → is-positive-ℤ (mul-ℤ x y)
is-positive-mul-ℤ {inr (inr zero-ℕ)} {inr (inr y)} H K = star
is-positive-mul-ℤ {inr (inr (succ-ℕ x))} {inr (inr y)} H K =
  is-positive-add-ℤ {inr (inr y)} K
    ( is-positive-mul-ℤ {inr (inr x)} {inr (inr y)} H K)

is-positive-abs-ℤ :
  (x : ℤ) → is-positive-ℤ x → is-positive-ℤ (int-abs-ℤ x)
is-positive-abs-ℤ (inr (inr x)) H = star

is-nonzero-abs-ℤ :
  (x : ℤ) → is-positive-ℤ x → is-nonzero-ℕ (abs-ℤ x)
is-nonzero-abs-ℤ (inr (inr x)) H = is-nonzero-succ-ℕ x

is-positive-int-ℕ :
  (x : ℕ) → is-nonzero-ℕ x → is-positive-ℤ (int-ℕ x)
is-positive-int-ℕ zero-ℕ H = ex-falso (H refl)
is-positive-int-ℕ (succ-ℕ x) H = star

-- Basics of nonnegative integers

nonnegative-ℤ : UU lzero
nonnegative-ℤ = Σ ℤ is-nonnegative-ℤ

int-nonnegative-ℤ : nonnegative-ℤ → ℤ
int-nonnegative-ℤ = pr1

is-nonnegative-int-nonnegative-ℤ :
  (x : nonnegative-ℤ) → is-nonnegative-ℤ (int-nonnegative-ℤ x)
is-nonnegative-int-nonnegative-ℤ = pr2

is-injective-int-nonnegative-ℤ : is-injective int-nonnegative-ℤ
is-injective-int-nonnegative-ℤ {pair (inr x) star} {pair (inr .x) star} refl =
  refl

is-nonnegative-int-ℕ : (n : ℕ) → is-nonnegative-ℤ (int-ℕ n)
is-nonnegative-int-ℕ zero-ℕ = star
is-nonnegative-int-ℕ (succ-ℕ n) = star

nonnegative-int-ℕ : ℕ → nonnegative-ℤ
pr1 (nonnegative-int-ℕ n) = int-ℕ n
pr2 (nonnegative-int-ℕ n) = is-nonnegative-int-ℕ n

nat-nonnegative-ℤ : nonnegative-ℤ → ℕ
nat-nonnegative-ℤ (pair (inr (inl x)) H) = zero-ℕ
nat-nonnegative-ℤ (pair (inr (inr x)) H) = succ-ℕ x

issec-nat-nonnegative-ℤ :
  (x : nonnegative-ℤ) → Id (nonnegative-int-ℕ (nat-nonnegative-ℤ x)) x
issec-nat-nonnegative-ℤ (pair (inr (inl star)) star) = refl
issec-nat-nonnegative-ℤ (pair (inr (inr x)) star) = refl

isretr-nat-nonnegative-ℤ :
  (n : ℕ) → Id (nat-nonnegative-ℤ (nonnegative-int-ℕ n)) n
isretr-nat-nonnegative-ℤ zero-ℕ = refl
isretr-nat-nonnegative-ℤ (succ-ℕ n) = refl

is-injective-nonnegative-int-ℕ : is-injective nonnegative-int-ℕ
is-injective-nonnegative-int-ℕ {x} {y} p =
  ( inv (isretr-nat-nonnegative-ℤ x)) ∙
  ( ( ap nat-nonnegative-ℤ p) ∙
    ( isretr-nat-nonnegative-ℤ y))

decide-is-nonnegative-ℤ :
  {x : ℤ} → coprod (is-nonnegative-ℤ x) (is-nonnegative-ℤ (neg-ℤ x))
decide-is-nonnegative-ℤ {inl x} = inr star
decide-is-nonnegative-ℤ {inr x} = inl star

-- We define the difference between two integers

diff-ℤ : ℤ → ℤ → ℤ
diff-ℤ x y = add-ℤ x (neg-ℤ y)

ap-diff-ℤ : {x x' y y' : ℤ} → Id x x' → Id y y' → Id (diff-ℤ x y) (diff-ℤ x' y')
ap-diff-ℤ p q = ap-binary diff-ℤ p q

eq-diff-ℤ : {x y : ℤ} → is-zero-ℤ (diff-ℤ x y) → Id x y
eq-diff-ℤ {x} {y} H =
  ( inv (right-unit-law-add-ℤ x)) ∙
  ( ( ap (add-ℤ x) (inv (left-inverse-law-add-ℤ y))) ∙
    ( ( inv (associative-add-ℤ x (neg-ℤ y) y)) ∙
      ( ( ap (add-ℤ' y) H) ∙
        ( left-unit-law-add-ℤ y))))

is-zero-diff-ℤ' : (x : ℤ) → is-zero-ℤ (diff-ℤ x x)
is-zero-diff-ℤ' x = right-inverse-law-add-ℤ x

is-zero-diff-ℤ :
  {x y : ℤ} → Id x y → is-zero-ℤ (diff-ℤ x y)
is-zero-diff-ℤ {x} {.x} refl = is-zero-diff-ℤ' x

left-zero-law-diff-ℤ : (x : ℤ) → Id (diff-ℤ zero-ℤ x) (neg-ℤ x)
left-zero-law-diff-ℤ x = left-unit-law-add-ℤ (neg-ℤ x)

right-zero-law-diff-ℤ : (x : ℤ) → Id (diff-ℤ x zero-ℤ) x
right-zero-law-diff-ℤ x = right-unit-law-add-ℤ x

left-successor-law-diff-ℤ :
  (x y : ℤ) → Id (diff-ℤ (succ-ℤ x) y) (succ-ℤ (diff-ℤ x y))
left-successor-law-diff-ℤ x y = left-successor-law-add-ℤ x (neg-ℤ y)

right-successor-law-diff-ℤ :
  (x y : ℤ) → Id (diff-ℤ x (succ-ℤ y)) (pred-ℤ (diff-ℤ x y))
right-successor-law-diff-ℤ x y =
  ap (add-ℤ x) (neg-succ-ℤ y) ∙ right-predecessor-law-add-ℤ x (neg-ℤ y)

left-predecessor-law-diff-ℤ :
  (x y : ℤ) → Id (diff-ℤ (pred-ℤ x) y) (pred-ℤ (diff-ℤ x y))
left-predecessor-law-diff-ℤ x y = left-predecessor-law-add-ℤ x (neg-ℤ y)

right-predecessor-law-diff-ℤ :
  (x y : ℤ) → Id (diff-ℤ x (pred-ℤ y)) (succ-ℤ (diff-ℤ x y))
right-predecessor-law-diff-ℤ x y =
  ap (add-ℤ x) (neg-pred-ℤ y) ∙ right-successor-law-add-ℤ x (neg-ℤ y)

triangle-diff-ℤ :
  (x y z : ℤ) → Id (add-ℤ (diff-ℤ x y) (diff-ℤ y z)) (diff-ℤ x z)
triangle-diff-ℤ x y z =
  ( associative-add-ℤ x (neg-ℤ y) (diff-ℤ y z)) ∙
  ( ap
    ( add-ℤ x)
    ( ( inv (associative-add-ℤ (neg-ℤ y) y (neg-ℤ z))) ∙
      ( ( ap (add-ℤ' (neg-ℤ z)) (left-inverse-law-add-ℤ y)) ∙
        ( left-unit-law-add-ℤ (neg-ℤ z)))))

distributive-neg-diff-ℤ :
  (x y : ℤ) → Id (neg-ℤ (diff-ℤ x y)) (diff-ℤ y x)
distributive-neg-diff-ℤ x y =
  ( distributive-neg-add-ℤ x (neg-ℤ y)) ∙
  ( ( ap (add-ℤ (neg-ℤ x)) (neg-neg-ℤ y)) ∙
    ( commutative-add-ℤ (neg-ℤ x) y))

interchange-law-add-diff-ℤ : interchange-law add-ℤ diff-ℤ
interchange-law-add-diff-ℤ x y u v =
  ( interchange-law-add-add-ℤ x (neg-ℤ y) u (neg-ℤ v)) ∙
  ( ap (add-ℤ (add-ℤ x u)) (inv (distributive-neg-add-ℤ y v)))

interchange-law-diff-add-ℤ : interchange-law diff-ℤ add-ℤ
interchange-law-diff-add-ℤ x y u v = inv (interchange-law-add-diff-ℤ x u y v)

left-translation-diff-ℤ :
  (x y z : ℤ) → Id (diff-ℤ (add-ℤ z x) (add-ℤ z y)) (diff-ℤ x y)
left-translation-diff-ℤ x y z =
  ( interchange-law-diff-add-ℤ z x z y) ∙
  ( ( ap (add-ℤ' (diff-ℤ x y)) (right-inverse-law-add-ℤ z)) ∙
    ( left-unit-law-add-ℤ (diff-ℤ x y)))

right-translation-diff-ℤ :
  (x y z : ℤ) → Id (diff-ℤ (add-ℤ x z) (add-ℤ y z)) (diff-ℤ x y)
right-translation-diff-ℤ x y z =
  ( ap-diff-ℤ (commutative-add-ℤ x z) (commutative-add-ℤ y z)) ∙
  ( left-translation-diff-ℤ x y z)

linear-diff-ℤ :
  (z x y : ℤ) → Id (diff-ℤ (mul-ℤ z x) (mul-ℤ z y)) (mul-ℤ z (diff-ℤ x y))
linear-diff-ℤ z x y =
  ( ap (add-ℤ (mul-ℤ z x)) (inv (right-negative-law-mul-ℤ z y))) ∙
  ( inv (left-distributive-mul-add-ℤ z x (neg-ℤ y)))

linear-diff-ℤ' :
  (x y z : ℤ) → Id (diff-ℤ (mul-ℤ x z) (mul-ℤ y z)) (mul-ℤ (diff-ℤ x y) z)
linear-diff-ℤ' x y z =
  ( ap (add-ℤ (mul-ℤ x z)) (inv (left-negative-law-mul-ℤ y z))) ∙
  ( inv (right-distributive-mul-add-ℤ x (neg-ℤ y) z))

-- We define the ordering of the integers

leq-ℤ : ℤ → ℤ → UU lzero
leq-ℤ x y = is-nonnegative-ℤ (diff-ℤ y x)

refl-leq-ℤ : (k : ℤ) → leq-ℤ k k
refl-leq-ℤ k = tr is-nonnegative-ℤ (inv (right-inverse-law-add-ℤ k)) star

antisymmetric-leq-ℤ : {x y : ℤ} → leq-ℤ x y → leq-ℤ y x → Id x y
antisymmetric-leq-ℤ {x} {y} H K =
  eq-diff-ℤ
    ( is-zero-is-nonnegative-ℤ K
      ( is-nonnegative-eq-ℤ (inv (distributive-neg-diff-ℤ x y)) H))

trans-leq-ℤ : (k l m : ℤ) → leq-ℤ k l → leq-ℤ l m → leq-ℤ k m
trans-leq-ℤ k l m p q =
  tr is-nonnegative-ℤ
    ( triangle-diff-ℤ m l k)
    ( is-nonnegative-add-ℤ
      ( add-ℤ m (neg-ℤ l))
      ( add-ℤ l (neg-ℤ k))
      ( q)
      ( p))

decide-leq-ℤ :
  {x y : ℤ} → coprod (leq-ℤ x y) (leq-ℤ y x)
decide-leq-ℤ {x} {y} =
  map-coprod
    ( id)
    ( is-nonnegative-eq-ℤ (distributive-neg-diff-ℤ y x))
    ( decide-is-nonnegative-ℤ {diff-ℤ y x})

succ-leq-ℤ : (k : ℤ) → leq-ℤ k (succ-ℤ k)
succ-leq-ℤ k =
  is-nonnegative-eq-ℤ
    ( inv
      ( ( left-successor-law-add-ℤ k (neg-ℤ k)) ∙
        ( ap succ-ℤ (right-inverse-law-add-ℤ k))))
    ( star)

leq-ℤ-succ-leq-ℤ : (k l : ℤ) → leq-ℤ k l → leq-ℤ k (succ-ℤ l)
leq-ℤ-succ-leq-ℤ k l p = trans-leq-ℤ k l (succ-ℤ l) p (succ-leq-ℤ l)

-- Bureaucracy

concatenate-eq-leq-eq-ℤ :
  {x' x y y' : ℤ} → Id x' x → leq-ℤ x y → Id y y' → leq-ℤ x' y'
concatenate-eq-leq-eq-ℤ refl H refl = H

concatenate-leq-eq-ℤ :
  (x : ℤ) {y y' : ℤ} → leq-ℤ x y → Id y y' → leq-ℤ x y'
concatenate-leq-eq-ℤ x H refl = H

concatenate-eq-leq-ℤ :
  {x x' : ℤ} (y : ℤ) → Id x' x → leq-ℤ x y → leq-ℤ x' y
concatenate-eq-leq-ℤ y refl H = H

-- The strict ordering on ℤ

le-ℤ : ℤ → ℤ → UU lzero
le-ℤ (inl zero-ℕ) (inl x) = empty
le-ℤ (inl zero-ℕ) (inr y) = unit
le-ℤ (inl (succ-ℕ x)) (inl zero-ℕ) = unit
le-ℤ (inl (succ-ℕ x)) (inl (succ-ℕ y)) = le-ℤ (inl x) (inl y)
le-ℤ (inl (succ-ℕ x)) (inr y) = unit
le-ℤ (inr x) (inl y) = empty
le-ℤ (inr (inl star)) (inr (inl star)) = empty
le-ℤ (inr (inl star)) (inr (inr x)) = unit
le-ℤ (inr (inr x)) (inr (inl star)) = empty
le-ℤ (inr (inr zero-ℕ)) (inr (inr zero-ℕ)) = empty
le-ℤ (inr (inr zero-ℕ)) (inr (inr (succ-ℕ y))) = unit
le-ℤ (inr (inr (succ-ℕ x))) (inr (inr zero-ℕ)) = empty
le-ℤ (inr (inr (succ-ℕ x))) (inr (inr (succ-ℕ y))) =
  le-ℤ (inr (inr x)) (inr (inr y))

--------------------------------------------------------------------------------

-- Extra material

-- We show that ℕ is an ordered semi-ring

left-law-leq-add-ℕ : (k m n : ℕ) → m ≤-ℕ n → (add-ℕ m k) ≤-ℕ (add-ℕ n k)
left-law-leq-add-ℕ zero-ℕ m n = id
left-law-leq-add-ℕ (succ-ℕ k) m n H = left-law-leq-add-ℕ k m n H

right-law-leq-add-ℕ : (k m n : ℕ) → m ≤-ℕ n → (add-ℕ k m) ≤-ℕ (add-ℕ k n) 
right-law-leq-add-ℕ k m n H =
  concatenate-eq-leq-eq-ℕ
    ( commutative-add-ℕ k m)
    ( left-law-leq-add-ℕ k m n H)
    ( commutative-add-ℕ n k)

preserves-leq-add-ℕ :
  {m m' n n' : ℕ} → m ≤-ℕ m' → n ≤-ℕ n' → (add-ℕ m n) ≤-ℕ (add-ℕ m' n')
preserves-leq-add-ℕ {m} {m'} {n} {n'} H K =
  transitive-leq-ℕ
    ( add-ℕ m n)
    ( add-ℕ m' n)
    ( add-ℕ m' n')
    ( left-law-leq-add-ℕ n m m' H)
    ( right-law-leq-add-ℕ m' n n' K)

--------------------------------------------------------------------------------

-- We prove some lemmas about inequalities --

leq-add-ℕ : (m n : ℕ) → m ≤-ℕ (add-ℕ m n)
leq-add-ℕ m zero-ℕ = refl-leq-ℕ m
leq-add-ℕ m (succ-ℕ n) =
  transitive-leq-ℕ m (add-ℕ m n) (succ-ℕ (add-ℕ m n))
    ( leq-add-ℕ m n)
    ( succ-leq-ℕ (add-ℕ m n))

leq-add-ℕ' : (m n : ℕ) → m ≤-ℕ (add-ℕ n m)
leq-add-ℕ' m n =
  concatenate-leq-eq-ℕ m (leq-add-ℕ m n) (commutative-add-ℕ m n)

leq-leq-add-ℕ :
  (m n x : ℕ) → (add-ℕ m x) ≤-ℕ (add-ℕ n x) → m ≤-ℕ n
leq-leq-add-ℕ m n zero-ℕ H = H
leq-leq-add-ℕ m n (succ-ℕ x) H = leq-leq-add-ℕ m n x H

leq-leq-add-ℕ' :
  (m n x : ℕ) → (add-ℕ x m) ≤-ℕ (add-ℕ x n) → m ≤-ℕ n
leq-leq-add-ℕ' m n x H =
  leq-leq-add-ℕ m n x
    ( concatenate-eq-leq-eq-ℕ
      ( commutative-add-ℕ m x)
      ( H)
      ( commutative-add-ℕ x n))

leq-leq-mul-ℕ :
  (m n x : ℕ) → (mul-ℕ (succ-ℕ x) m) ≤-ℕ (mul-ℕ (succ-ℕ x) n) → m ≤-ℕ n
leq-leq-mul-ℕ zero-ℕ zero-ℕ x H = star
leq-leq-mul-ℕ zero-ℕ (succ-ℕ n) x H = star
leq-leq-mul-ℕ (succ-ℕ m) zero-ℕ x H =
  ex-falso
    ( concatenate-leq-eq-ℕ
      ( mul-ℕ (succ-ℕ x) (succ-ℕ m))
      ( H)
      ( right-zero-law-mul-ℕ (succ-ℕ x)))
leq-leq-mul-ℕ (succ-ℕ m) (succ-ℕ n) x H =
  leq-leq-mul-ℕ m n x
    ( leq-leq-add-ℕ' (mul-ℕ (succ-ℕ x) m) (mul-ℕ (succ-ℕ x) n) (succ-ℕ x)
      ( concatenate-eq-leq-eq-ℕ
        ( inv (right-successor-law-mul-ℕ (succ-ℕ x) m))
        ( H)
        ( right-successor-law-mul-ℕ (succ-ℕ x) n)))

leq-leq-mul-ℕ' :
  (m n x : ℕ) → (mul-ℕ m (succ-ℕ x)) ≤-ℕ (mul-ℕ n (succ-ℕ x)) → m ≤-ℕ n
leq-leq-mul-ℕ' m n x H =
  leq-leq-mul-ℕ m n x
    ( concatenate-eq-leq-eq-ℕ
      ( commutative-mul-ℕ (succ-ℕ x) m)
      ( H)
      ( commutative-mul-ℕ n (succ-ℕ x)))

{-
succ-relation-ℕ :
  {i : Level} (R : ℕ → ℕ → UU i) → ℕ → ℕ → UU i
succ-relation-ℕ R m n = R (succ-ℕ m) (succ-ℕ n)

succ-reflexivity-ℕ :
  {i : Level} (R : ℕ → ℕ → UU i) (ρ : (n : ℕ) → R n n) →
  (n : ℕ) → succ-relation-ℕ R n n
succ-reflexivity-ℕ R ρ n = ρ (succ-ℕ n)

{- In the book we suggest that first the order of the variables should be
   swapped, in order to make the inductive hypothesis stronger. Agda's pattern
   matching mechanism allows us to bypass this step and give a more direct
   construction. -}

least-reflexive-Eq-ℕ :
  {i : Level} (R : ℕ → ℕ → UU i) (ρ : (n : ℕ) → R n n) →
  (m n : ℕ) → Eq-ℕ m n → R m n
least-reflexive-Eq-ℕ R ρ zero-ℕ zero-ℕ star = ρ zero-ℕ
least-reflexive-Eq-ℕ R ρ zero-ℕ (succ-ℕ n) ()
least-reflexive-Eq-ℕ R ρ (succ-ℕ m) zero-ℕ ()
least-reflexive-Eq-ℕ R ρ (succ-ℕ m) (succ-ℕ n) e =
  least-reflexive-Eq-ℕ (succ-relation-ℕ R) (succ-reflexivity-ℕ R ρ) m n e
-}

{-
--------------------------------------------------------------------------------

data Fin-Tree : UU lzero where
  constr : (n : ℕ) → (Fin n → Fin-Tree) → Fin-Tree

root-Fin-Tree : Fin-Tree
root-Fin-Tree = constr zero-ℕ ex-falso

succ-Fin-Tree : Fin-Tree → Fin-Tree
succ-Fin-Tree t = constr one-ℕ (λ i → t)

map-assoc-coprod :
  {l1 l2 l3 : Level} {A : UU l1} {B : UU l2} {C : UU l3} →
  coprod (coprod A B) C → coprod A (coprod B C)
map-assoc-coprod (inl (inl x)) = inl x
map-assoc-coprod (inl (inr x)) = inr (inl x)
map-assoc-coprod (inr x) = inr (inr x)

map-coprod-Fin :
  (m n : ℕ) → Fin (add-ℕ m n) → coprod (Fin m) (Fin n)
map-coprod-Fin m zero-ℕ = inl
map-coprod-Fin m (succ-ℕ n) =
  map-assoc-coprod ∘ (map-coprod (map-coprod-Fin m n) (id {A = unit}))

add-Fin-Tree : Fin-Tree → Fin-Tree → Fin-Tree
add-Fin-Tree (constr n x) (constr m y) =
  constr (add-ℕ n m) ((ind-coprod (λ i → Fin-Tree) x y) ∘ (map-coprod-Fin n m))

--------------------------------------------------------------------------------

data labeled-Bin-Tree {l1 : Level} (A : UU l1) : UU l1 where
  leaf : A → labeled-Bin-Tree A
  constr : (bool → labeled-Bin-Tree A) → labeled-Bin-Tree A

mul-leaves-labeled-Bin-Tree :
  {l1 : Level} {A : UU l1} (μ : A → (A → A)) →
  labeled-Bin-Tree A → A
mul-leaves-labeled-Bin-Tree μ (leaf x) = x
mul-leaves-labeled-Bin-Tree μ (constr f) =
  μ ( mul-leaves-labeled-Bin-Tree μ (f false))
    ( mul-leaves-labeled-Bin-Tree μ (f true))

pick-list : {l1 : Level} {A : UU l1} → ℕ → list A → coprod A unit
pick-list zero-ℕ nil = inr star
pick-list zero-ℕ (cons a x) = inl a
pick-list (succ-ℕ n) nil = inr star
pick-list (succ-ℕ n) (cons a x) = pick-list n x
-}
```
